Download Link: https://assignmentchef.com/product/solved-dynamical-homework-10
<br>
<strong>1.1      Section 4.6 Problem 2.</strong>

Observe that <em>|f| </em>is defined as,



<em>f</em>(<em>x</em>)           if <em>f</em>(<em>x</em>) <em>≥ </em>0

<em>|f| </em>=

<em>−f</em>(<em>x</em>)         if <em>f</em>(<em>x</em>) <em>&lt; </em>0

In addition, we have,



<sub>+          </sub><em>f</em>(<em>x</em>)        if <em>f</em>(<em>x</em>) <em>≥ </em>0

<em>f     </em>=

0            if <em>f</em>(<em>x</em>) <em>&lt; </em>0

and,



<em>f</em><em>− </em>= <em>−f</em>(<em>x</em>)          if <em>f</em>(<em>x</em>) <em>≤ </em>0

0               if <em>f</em>(<em>x</em>) <em>&gt; </em>0

Now let us consider <em>f</em><sup>+</sup>(<em>x</em>) + <em>f<sup>−</sup></em>(<em>x</em>) for 3 cases: when <em>f</em>(<em>x</em>) <em>&gt; </em>0, when <em>f</em>(<em>x</em>) = 0, and when <em>f</em>(<em>x</em>) <em>&lt; </em>0. When <em>f</em>(<em>x</em>) <em>&gt; </em>0, we have that <em>f</em><sup>+</sup>(<em>x</em>) = <em>f</em>(<em>x</em>) and <em>f<sup>−</sup></em>(<em>x</em>) = 0. Hence, <em>f</em><sup>+</sup>(<em>x</em>) + <em>f<sup>−</sup></em>(<em>x</em>) = <em>f</em>(<em>x</em>) in this case, just as in the case of <em>|f|</em>. Now suppose <em>f</em>(<em>x</em>) = 0. Then <em>f</em><sup>+</sup>(<em>x</em>) = 0 and <em>f<sup>−</sup></em>(<em>x</em>) = 0, so <em>f</em><sup>+</sup>(<em>x</em>) + <em>f<sup>−</sup></em>(<em>x</em>) = 0. Again, <em>|f</em>(<em>x</em>)<em>| </em>= 0 when <em>f</em>(<em>x</em>) = 0, so they coincide in this case as well. Now suppose <em>f</em>(<em>x</em>) <em>&lt; </em>0. Then <em>f</em><sup>+</sup>(<em>x</em>) = 0 and <em>f<sup>−</sup></em>(<em>x</em>) = <em>−f</em>(<em>x</em>). Thus, <em>f</em><sup>+</sup>(<em>x</em>) + <em>f<sup>−</sup></em>(<em>x</em>) = <em>−f</em>(<em>x</em>). This is precisely the same as <em>|f|</em>. Hence, in all 3 possible cases for <em>f</em>(<em>x</em>), we have that <em>f</em><sup>+ </sup>+ <em>f<sup>− </sup></em>coincides with <em>|f|</em>, and so <em>f</em><sup>+ </sup>+ <em>f<sup>− </sup></em>= <em>|f|</em>.

<strong>Problem 3.</strong>

Suppose <em>f </em>is integrable. Then <sup>R </sup><em>f</em><sup>+</sup><em>dµ &lt; ∞ </em>and <sup>R </sup><em>f<sup>−</sup>dµ &lt; ∞</em>. Hence, <sup>R </sup><em>f</em><sup>+</sup><em>dµ</em>+<sup>R </sup><em>f<sup>−</sup>dµ &lt; ∞</em>. By Lemma 4.6.2 Part 2, we have that,

Z                      Z                      Z

<em>f</em><sup>+</sup><em>dµ </em>+        <em>f<sup>−</sup>dµ </em>=         (<em>f</em><sup>+ </sup>+ <em>f<sup>−</sup></em>)<em>dµ</em>

<em>&lt; ∞</em>

By Exercise 2, we thus have that,

<h2>                                                                           Z                                      Z</h2>

+           <em>−</em>

(<em>f       </em>+ <em>f </em>)<em>dµ </em>=        <em>|f|dµ</em>

<em>&lt; ∞</em>

Now suppose <em>|f| </em>is integrable. Then <sup>R </sup><em>|f|</em><sup>+</sup><em>dµ &lt; ∞ </em>and <sup>R </sup><em>|f|<sup>−</sup>dµ &lt; ∞</em>. But observe that, since <em>|f| ≥ </em>0 everywhere, then <em>|f|<sup>− </sup></em>= 0 everywhere. Hence, we from this and our work in Exercise 2 that,

<h2>                                                                    Z                      Z                         Z</h2>

<em>|f|dµ </em>=       <em>|f|</em><sup>+</sup><em>dµ −      |f|<sup>−</sup>dµ</em>

Z

=      <em>|f|</em><sup>+</sup><em>dµ</em>

Z

=        (<em>f</em><sup>+ </sup><em>− f<sup>−</sup></em>)<em>dµ</em>

Then, by Lemma 4.6.2 Part 2, we have that <em>f</em><sup>+ </sup>and <em>f<sup>− </sup></em>are integrable and thus, <sup>R </sup><em>f</em><sup>+</sup><em>dµ &lt; ∞ </em>and <sup>R </sup><em>f<sup>−</sup>dµ &lt; ∞</em>. Hence,

Z                      Z

<em>f</em><sup>+</sup><em>dµ −         f<sup>−</sup>dµ &lt; ∞</em>

And thus, we have that <sup>R </sup><em>fdµ </em>= <sup>R </sup><em>f</em><sup>+</sup><em>dµ − </em><sup>R </sup><em>f<sup>−</sup>dµ </em>is integrable, as required.

<strong>Problem 4.</strong>

Suppose <em>f </em>is an integrable function and fix <em>a ∈ </em>R. We have that,

<h2>                                                                         Z                   Z                      Z</h2>

<em>fdµ </em>=        <em>f</em><sup>+</sup><em>dµ −        f<sup>−</sup>dµ</em>

with <sup>R </sup><em>f</em><sup>+</sup><em>dµ &lt; ∞ </em>and <sup>R </sup><em>f<sup>−</sup>dµ &lt; ∞</em>. Observe that <em>f</em><sup>+</sup><em>,f<sup>− </sup></em>are thus nonnegative integrable functions. Thus, applying Theorem 4.4.5, we have that, <em>af</em><sup>+ </sup>and <em>af<sup>− </sup></em>are integrable. Thus,

<sup>R </sup><em>af</em><sup>+</sup><em>dµ &lt; ∞ </em>and <sup>R </sup><em>af<sup>−</sup>dµ &lt; ∞ </em>and so,

Z                         Z

+                         <em>−</em>

<em>af dµ −         af dµ &lt; ∞</em>

But the above is precisely the definition of <sup>R </sup><em>afdµ</em>, and so we must have that <em>af </em>is integrable.

<strong>Problem 5.</strong>

Suppose that <em>f ≤ g </em>a.e. Then of course <em>f</em><sup>+ </sup><em>≤ g</em><sup>+ </sup>a.e. If this were not the case, then there would be a set of positive measure on which <em>f</em><sup>+ </sup><em>&gt; g</em><sup>+</sup>, which, by the definition of <em>f</em><sup>+ </sup>and <em>g</em><sup>+</sup>, would imply that there is a set of positive measure on which <em>f &gt; g</em>, a contradiction.

In addition, we have that <em>f<sup>− </sup>≥ g<sup>− </sup></em>a.e. Suppose that this is not the case. Then there is a set of positive measure on which <em>f<sup>− </sup>&lt; g<sup>−</sup></em>. But this implies that <em>f</em>(<em>x</em>) <em>&gt; g</em>(<em>x</em>) for <em>x </em>in this set (either <em>f</em>(<em>x</em>) <em>≥ </em>0 or <em>f</em>(<em>x</em>) is a negative number greater than <em>g</em>(<em>x</em>)). This is a contradiction, and so we must have <em>f<sup>− </sup>≥ g<sup>− </sup></em>a.e. Hence, we have that,

<h2>                                                                         Z                   Z                      Z</h2>

+                      <em>−</em>

<em>fdµ </em>=        <em>f dµ −        f dµ</em>

where <em>f</em><sup>+ </sup><em>≤ g</em><sup>+ </sup>a.e. and <em>f<sup>− </sup>≥ g<sup>− </sup></em>a.e. Now let us consider <sup>R </sup><em>f</em><sup>+</sup><em>dµ </em>and <sup>R </sup><em>g</em><sup>+</sup><em>dµ</em>. We have,

Z       Z


<em>f dµ </em>= sup<em>{             sdµ </em>: <em>s </em>is simple and 0 <em>≤ s ≤ f }</em>

Z       Z


<em>g dµ </em>= sup<em>{            sdµ </em>: <em>s<sub>g </sub></em>is simple and 0 <em>≤ s ≤ g }</em>

We have that <em>f</em><sup>+ </sup><em>≤ g</em><sup>+ </sup>a.e. Let <em>s<sub>g </sub></em>be the supremum of simple function in the above set, and the same for <em>s<sub>f</sub></em>. Then we must have <em>s<sub>f </sub>≤ s<sub>g </sub></em>a.e. as well. Observe that the set <em>X </em>where <em>s<sub>f </sub>&gt; s<sub>g </sub></em>is measure 0, and so it does contribute at all to the value of the integral by Corollary 4.3.3. Thus, we can disregard <em>X </em>when calculating the integral and so apply Theorem 4.3.2(2) which states that,

<h2>                                                                                     Z                     Z</h2>

<em>s<sub>f</sub>dµ ≤       s<sub>g</sub>dµ</em>

Since these were the supremum of simple functions approximating <em>f</em><sup>+ </sup>and <em>g</em><sup>+</sup>, we have

that,

<h2>                                                                                   Z                       Z</h2>




<em>f dµ ≤        g dµ</em>

Similarly, we have that,

<h2>                                                                                   Z                       Z</h2>

<em>−                      −</em>

<em>f dµ ≥        g dµ</em>

These two inequalities and the fact that all of these integrals are nonnegative give us that,

Z                   Z                      Z                      Z                      Z                      Z

+                      <em>−                      </em>+                     <em>−</em>

<em>fdµ </em>=        <em>f dµ −         f dµ ≤        g dµ −        g dµ </em>=       <em>gdµ</em>

as required.

<strong>Problem 6.</strong>

Let <em>f </em>be an integrable function and suppose that <sup>R</sup><em><sub>A </sub>fdµ </em>= 0 for all measurable sets <em>A</em>. Then we have,

Z                       Z

+                       <em>−</em>

<em>f dµ −          f dµ </em>= 0

<em>A                       A</em>

Since both of the above integrals are nonnegative, we must have that <sup>R</sup><em><sub>A </sub>f</em><sup>+</sup><em>dµ </em>= 0 = <sup>R </sup><em>f<sup>−</sup>dµ</em>. Since <em>f</em><sup>+ </sup>and <em>f<sup>− </sup></em>are both nonnegative measurable functions, by Problem 4.4.2

<em><sub>A</sub></em>

(solved on the previous HW), we have that <em>f</em><sup>+ </sup>= 0 a.e. and <em>f<sup>− </sup></em>= 0 a.e. on <em>A</em>. Let <em>X </em>be the set where <em>f</em><sup>+ </sup><em>&gt; </em>0 and <em>Y </em>be the set where <em>f<sup>− </sup>&gt; </em>0 and let <em>Z </em>= <em>X ∪ Y </em>. Then <em>µ</em>(<em>Z</em>) <em>≤ µ</em>(<em>X</em>) + <em>µ</em>(<em>Y </em>) = 0 + 0 = 0. Note that <em>Z </em>is precisely the set where <em>f 6</em>= 0 (since when <em>f </em>= 0 we have <em>f</em><sup>+ </sup>= <em>f<sup>− </sup></em>= 0 and when <em>f 6</em>= 0, one of <em>f</em><sup>+ </sup>and <em>f<sup>− </sup></em>is greater than 0). Hence, the set of values where <em>f 6</em>= 0 on <em>A </em>has measure 0 and so <em>f </em>= 0 a.e. on <em>A</em>.

<strong>Problem 7.</strong>

Suppose <em>f </em>is a nonnegative integrable function and that <em>{E<sub>p</sub>}<sub>p&gt;</sub></em><sub>0 </sub>is a sequence of decreasing (<em>E<sub>p</sub></em><sub>+1 </sub><em>⊂ E<sub>p</sub></em>) measurable sets. Furthermore, suppose lim<em><sub>p→∞ </sub>µ</em>(<em>E<sub>p</sub></em>) = 0. We want to show that Z

<em>fdµ </em>= 0

<em>∩</em><em>p&gt;</em>0<em>E</em><em>p</em>

We know that since lim<em><sub>p→∞ </sub>µ</em>(<em>E<sub>p</sub></em>) = 0 that for every <em> &gt; </em>0, there exists <em>N ∈ </em>N such that for all <em>n &gt; N</em>, we have that <em>|E<sub>n</sub>| &lt; </em>. Observe that since we have a decreasing sequence of sets, for any finite subset <em>{E</em><sub>0</sub><em>,E</em><sub>1</sub><em>,…,E<sub>k</sub>}</em>, we have that<em> E<sub>k </sub></em>and so <em>µ∩<sub>i</sub><sup>k</sup></em><sub>=0</sub><em>E<sub>i</sub></em> = <em>µ</em>(<em>E<sub>k</sub></em>). Thus, by Proposition 2.5.2(2), we have

<em>µ</em>(<em>∩<sub>p&gt;</sub></em><sub>0</sub><em>E<sub>p</sub></em>) = lim <em>µ</em>(<em>E<sub>p</sub></em>)

<em>p→∞</em>

= 0

Note that since <em>µ</em>(<em>∩<sub>p&gt;</sub></em><sub>0</sub><em>E<sub>p</sub></em>), any measurable subset of <em>∩<sub>p&gt;</sub></em><sub>0</sub><em>E<sub>p </sub></em>must have measure 0 as well. Thus, for any simple function <em>s </em>defined on <em>µ</em>(<em>∩<sub>p&gt;</sub></em><sub>0</sub><em>E<sub>p</sub></em>), we have that <em>s </em>= 0. But this implies that <sup>R</sup><em><sub>∩</sub></em><em><sub>p&gt;</sub></em><sub>0<em>E</em></sub><em><sub>p </sub>sdµ </em>for all simple functions <em>s </em>by the formulation of the integral given by Corollary 4.3.3. But if the integral of any simple function on <em>∩<sub>p&gt;</sub></em><sub>0</sub><em>E<sub>p </sub></em>is 0, then we have that the integral of non-negative simple function must be 0 as well because, for a nonnegative function <em>g</em>,

Z                                         Z

<em>gdµ </em>= sup<em>{                   sdµ </em>: <em>s </em>is simple and 0 <em>≤ s ≤ g}</em>

<em>∩</em><em>p&gt;</em>0<em>E</em><em>p                                                  </em><em>∩</em><em>p&gt;</em>0<em>E</em><em>p</em>

= sup<em>{</em>0<em>}</em>

= 0

Since <em>f</em><sup>+ </sup>and <em>f<sup>− </sup></em>are nonnegative measurable functions defined on <em>∩<sub>p&gt;</sub></em><sub>0</sub><em>E<sub>p</sub></em>, we have that

Z                                            Z

+                                           <em>−</em>

<em>f dµ </em>= 0 =                  <em>f dµ</em>

<em>∩</em><em>p&gt;</em>0<em>E</em><em>p                                                      </em><em>∩</em><em>p&gt;</em>0<em>E</em><em>p</em>

And, hence,

Z                               Z                                  Z

+                                 <em>−</em>

<em>fdµ </em>=                 <em>f dµ −                 f dµ</em>

<em>∩</em><em>p&gt;</em>0<em>E</em><em>p                        </em><em>∩</em><em>p&gt;</em>0<em>E</em><em>p     </em><em>∩</em><em>p&gt;</em>0<em>E</em><em>p </em>= 0 <em>− </em>0 = 0

as required.

<strong>Problem 9.</strong>

Let <em>f </em>: <em>X → </em>R<em><sup>∗ </sup></em>be a measurable function and <em>f </em>is integrable. Now suppose <em>|f</em>(<em>x</em>)<em>| </em>= <em>∞ </em>on a set <em>X </em>with <em>µ</em>(<em>X</em>) <em>&gt; </em>0. Then <em>f </em>= <em>∞ </em>or <em>f </em>= <em>−∞ </em>(or both) on a set of positive measure. Thus, we have that either <em>f</em><sup>+ </sup>= <em>∞ </em>or <em>f<sup>− </sup></em>= <em>∞ </em>(or both) on a set of positive measure. Thus, a maximal <em>s </em>approximating simple function on <em>f</em><sup>+ </sup>or <em>f<sup>− </sup></em>(or both) must attain <em>∞ </em>on a set of positive measure. Hence, we have <em>s </em>= <sup>P<em>n </em></sup><em>a<sub>i</sub>µ</em>(<em>A<sub>i</sub></em>) = <em>a</em><sub>0</sub><em>µ</em>(<em>A</em><sub>0</sub>)+<em>a</em><sub>1</sub><em>µ</em>(<em>A</em><sub>1</sub>)+<em>···</em>+<em>∞µ</em>(<em>A<sub>k</sub></em>)+ <em>··· </em>+ <em>a<sub>n</sub>µ</em>(<em>A<sub>n</sub></em>) = <em>∞</em>. Since <em>∞ </em>is the max value attainable in R<em><sup>∗ </sup></em>it must be the supremum of any subset of R<em><sup>∗ </sup></em>containing it, and so,

Z       Z


<em>f dµ </em>= sup<em>{             sdµ </em>: <em>s </em>is simple and 0 <em>≤ s ≤ f }</em>

= <em>∞</em>

or,

Z                                 Z

<em>−                                                                                                        −</em>

<em>f dµ </em>= sup<em>{             sdµ </em>: <em>s </em>is simple and 0 <em>≤ s ≤ f }</em>

= <em>∞</em>

or both. But note that <em>f </em>is only Lebesgue integrable if both <sup>R </sup><em>f</em><sup>+ </sup><em>&lt; ∞ </em>and <sup>R </sup><em>f<sup>− </sup>&lt; ∞</em>. Hence, we have that <em>f </em>is not integrable, a contradiction. Thus, we must have that the set where <em>|f</em>(<em>x</em>)<em>| </em>= <em>∞ </em>has measure 0. That is, <em>|f</em>(<em>x</em>)<em>| &lt; ∞ </em>a.e.